# 忘却関数

$$Q_{(n,t)}=C_{(n,t)}+(1-C_{(n,t)})*e^{-\frac {t}{α_{(n)}}}$$

$Q_{(n,t)}$ ： 忘却関数

$C_{(n,t)}$ ： 前回正答分の忘却関数

$α_{(n)}$ ： 仮忘却時定数

$t$ ： 前回学習からの日数

## 前回正答分の忘却関数

前回正答分の忘却関数を次の様に表す

$$C_{(n,t)}=Z_{(n)}*e^{-\frac {t}{β_{(n)}}}$$

$Z_{(n)}$ ： 前回正答率

$β_{(n)}$ ： 前回正答忘却時定数

### 結合

$Q_{(n,t)}=C_{(n,t)}+(1-C_{(n,t)})*e^{-\frac {t}{α_{(n)}}}$

$C_{(n,t)}=Z_{(n)}*e^{-\frac {t}{β_{(n)}}}$

$Q_{(n,t)}=Z_{(n)}*e^{-\frac {t}{β_{(n)}}}+(1-Z_{(n)}*e^{-\frac {t}{β_{(n)}}})*e^{-\frac {t}{α_{(n)}}}$

### 仮忘却時定数

$e^{-\frac {t}{α_{(n)}}}=\frac{Q_{(n,t)}-Z_{(n)}*e^{-\frac {t}{β_{(n)}}}}{1-Z_{(n)}*e^{-\frac {t}{β_{(n)}}}}$

$M=Z_{(n)}*e^{-\frac {t}{β_{(n)}}}$

$log(e^{-\frac {t}{α_{(n)}}})=log(\frac{Q_{(n,t)}-M}{1-M})$

$-\frac {t}{α_{(n)}}=log(\frac{Q_{(n,t)}-M}{1-M})$

$-\frac {t}{log(\frac{Q_{(n,t)}-M}{1-M})}=α_(n)$

## 時定数

$β_{(n)}=β_{(n-1)}e^{1.25}$

$β_{(0)}=1$

---

$Q_{(n,t)}=e^{-\frac {t}{α_{(n)}}}$

$e^{-\frac {t}{α_{(n)}}}=Q_{(n,t)}$

$log(e^{-\frac {t}{α_{(n)}}})=log(Q_{(n,t)})$

$-\frac {t}{α_{(n)}}=log(Q_{(n,t)})$

$-\frac {t}{log(Q_{(n,t)})}=α_{(n)}$
